Fixed TlsAux according to weaker iord_simpl lemmas in IMM; minimized WFSC usage

src/tls_props/TlsAux.v
@@ -36,7 +36,9 @@ Section TlsProperties.
   Variable WF : Wf G.
   Variable COM : complete G.
   Variable sc : relation actid.
-  Variable IMMCON : imm_consistent G sc.
+  (* Variable IMMCON : imm_consistent G sc. *)
+  Variable WFSC: wf_sc G sc. 
+  Variable SCPL: sc_per_loc G. 
 
   Notation "'sb'" := (sb G).
   Notation "'rmw'" := (rmw G).
@@ -181,35 +183,42 @@ Definition issuable T :=
     splits; eauto.
   Qed.
 
-  (* TODO: move somewhere *)
-  Lemma dom_rel_iord_parts (a1 a2: trav_action) (r: relation actid)
-        (R_IORD: ⦗action ↓₁ eq a1⦘ ⨾ event ↓ r ⨾ ⦗action ↓₁ eq a2⦘
-                 ⊆ iord_simpl G sc):
-    dom_rel (r ⨾ ⦗event ↑₁ (T ∩₁ action ↓₁ eq a2)⦘)
-    ⊆₁ event ↑₁ (T ∩₁ action ↓₁ eq a1).
-  Proof using WF TLSCOH IORDCOH IMMCON. 
-    eapply dom_rel_collect_event with (b := a1); [basic_solver| ].
-    apply set_subset_inter_r. split; [| basic_solver].
-    rewrite set_interC, id_inter. sin_rewrite R_IORD.
-    eapply iord_coh_implies_iord_simpl_coh; eauto.
-  Qed.
+  (* Lemma dom_rel_iord_parts (a1 a2: trav_action) (r: relation actid) *)
+  (*       (R_IORD: ⦗action ↓₁ eq a1⦘ ⨾ event ↓ r ⨾ ⦗action ↓₁ eq a2⦘ *)
+  (*                ⊆ iord_simpl G sc) *)
+  (*       (R_E_ENI: r ⊆ E × (E \₁ is_init)): *)
+  (*   dom_rel (r ⨾ ⦗event ↑₁ (T ∩₁ action ↓₁ eq a2)⦘) *)
+  (*   ⊆₁ event ↑₁ (T ∩₁ action ↓₁ eq a1). *)
+  (* (* TODO: move somewhere *) *)
+  (* Lemma dom_rel_iord_parts (a1 a2: trav_action) (r: relation actid) *)
+  (*       (R_IORD: ⦗action ↓₁ eq a1⦘ ⨾ event ↓ r ⨾ ⦗action ↓₁ eq a2⦘ *)
+  (*                ⊆ iord_simpl G sc): *)
+  (*   dom_rel (r ⨾ ⦗event ↑₁ (T ∩₁ action ↓₁ eq a2)⦘) *)
+  (*   ⊆₁ event ↑₁ (T ∩₁ action ↓₁ eq a1). *)
+  (* Proof using WF TLSCOH IORDCOH WFSC SCPL.  *)
+  (*   eapply dom_rel_collect_event with (b := a1); [basic_solver| ]. *)
+  (*   apply set_subset_inter_r. split; [| basic_solver]. *)
+  (*   rewrite set_interC, id_inter. sin_rewrite R_IORD. *)
+  (*   eapply iord_coh_implies_iord_simpl_coh'; eauto. *)
+  (* Qed. *)
+
+  Lemma iord_alt:
+    iord G sc ≡ restr_rel (event ↓₁ (E \₁ is_init)) (iord_simpl G sc).
+  Proof using. unfold iord, iord_simpl. basic_solver 10. Qed.
 
   Lemma dom_cond_alt {A : Type} (r : relation A) (d : A -> Prop):
     dom_cond r d ≡₁ (⋃₁ e ∈ (fun e_ => dom_rel (r ⨾ ⦗eq e_⦘) ⊆₁ d), eq e).
   Proof using. unfold dom_cond. basic_solver 10. Qed. 
   
-  Lemma iord_alt:
-    iord G sc ≡ restr_rel (event ↓₁ (E \₁ is_init)) (iord_simpl G sc).
-  Proof using. unfold iord, iord_simpl. basic_solver 10. Qed.
-
-  Lemma iord_simpl_irreflexive:
+  Lemma iord_simpl_irreflexive (IMMCON: imm_consistent G sc):
     irreflexive (iord_simpl G sc). 
-  Proof using WF IMMCON COM. 
+  Proof using WF COM.
+    clear WFSC. 
     unfold iord_simpl.
     repeat (apply irreflexive_union; split).
     all: auto using SB_irr, RF_irr, FWBOB_irr, AR_irr, IPROP_irr, PROP_irr.
-    apply SB_irr; auto. apply IMMCON.
-  Qed. 
+    apply SB_irr; auto. by apply IMMCON. 
+  Qed.
 
   (* TODO: move somewhere *)
   Lemma dom_rel_iord_ext_parts (a1 a2: trav_action) (r: relation actid)
@@ -277,7 +286,7 @@ Definition issuable T :=
 
   Lemma sb_covered :
     sb ⨾ ⦗ covered T ⦘ ≡ ⦗ covered T ⦘ ⨾ sb ⨾ ⦗ covered T ⦘.
-  Proof using WF TLSCOH IORDCOH IMMCON.
+  Proof using WF TLSCOH IORDCOH .
     rewrite (dom_rel_helper dom_sb_covered). basic_solver.
   Qed.
 
@@ -314,38 +323,37 @@ Definition issuable T :=
 
   Lemma dom_sc_coverable :
     dom_rel (sc ⨾ ⦗ coverable T ⦘) ⊆₁ covered T.
-  Proof using WF TLSCOH IMMCON.
+  Proof using WF TLSCOH WFSC.
     unfold coverable, covered. rewrite id_inter, <- seqA.
-    cdes IMMCON. 
     apply dom_rel_iord_ext_parts.
     3: by apply init_covered.
-    2: { erewrite (sc_E_ENI _ _ WF Wf_sc). basic_solver. } 
+    2: { erewrite (sc_E_ENI _ _ WF WFSC). basic_solver. } 
     transitivity (SB G sc); [| unfold iord_simpl; basic_solver 10].
     unfold SB. hahn_frame. apply map_rel_mori; [done| ].
-    rewrite <- ct_step. rewrite (wf_scE Wf_sc). basic_solver 10.
+    rewrite <- ct_step. rewrite (wf_scE WFSC). basic_solver 10.
   Qed. 
     
   Lemma dom_sc_covered :
     dom_rel (sc ⨾ ⦗ covered T ⦘) ⊆₁ covered T.
-  Proof using WF TLSCOH IORDCOH IMMCON. 
+  Proof using WF TLSCOH IORDCOH WFSC. 
     rewrite covered_in_coverable at 1. apply dom_sc_coverable. 
   Qed.
 
   Lemma sc_coverable  :
     sc ⨾ ⦗ coverable T ⦘ ⊆ ⦗covered T⦘ ⨾ sc.
-  Proof using WF TLSCOH IMMCON.
+  Proof using WF TLSCOH WFSC.
     seq_rewrite (dom_rel_helper dom_sc_coverable). basic_solver.
   Qed.
 
   Lemma sc_covered :
     sc ⨾ ⦗covered T⦘ ⊆ ⦗covered T⦘ ⨾ sc.
-  Proof using WF TLSCOH IORDCOH IMMCON. 
+  Proof using WF TLSCOH IORDCOH WFSC. 
     seq_rewrite (dom_rel_helper dom_sc_covered). basic_solver.
   Qed.
 
   Lemma ar_coverable_in_CI  :
     dom_rel (ar ⨾ ⦗coverable T⦘) ⊆₁ covered T ∪₁ issued T.
-  Proof using WF TLSCOH IORDCOH IMMCON.
+  Proof using WF TLSCOH IORDCOH WFSC.
     unfold imm_s.ar.
     rewrite !seq_union_l.
     rewrite ar_int_in_sb, rfe_in_rf; eauto. 
@@ -355,7 +363,7 @@ Definition issuable T :=
 
   Lemma ar_C_in_CI  :
     dom_rel (ar ⨾ ⦗covered T⦘) ⊆₁ covered T ∪₁ issued T.
-  Proof using WF TLSCOH IORDCOH IMMCON.
+  Proof using WF TLSCOH IORDCOH WFSC.
     unfold imm_s.ar.
     rewrite !seq_union_l.
     rewrite (ar_int_in_sb WF).
@@ -368,7 +376,7 @@ Definition issuable T :=
   (* TODO: move to IordCoherency *)
   Lemma ar_rf_ppo_loc_ct_E_ENI: 
     (ar ∪ rf ⨾ ppo ∩ same_loc)⁺ ⊆ E × (E \₁ Init).
-  Proof using WF IMMCON. 
+  Proof using WF WFSC. 
     rewrite inclusion_inter_l1, ppo_in_sb; auto. 
     rewrite sb_E_ENI, rf_E_ENI, ar_E_ENI; auto.
     remember (E × (E \₁ Init)) as E_ENI. 
@@ -381,7 +389,7 @@ Definition issuable T :=
 
   Lemma ar_rf_ppo_loc_ct_issuable_in_I  :
     dom_rel (⦗W⦘ ⨾ (ar ∪ rf ⨾ (ppo ∩ same_loc))⁺ ⨾ ⦗issuable T⦘) ⊆₁ issued T.
-  Proof using WF TLSCOH IMMCON.
+  Proof using WF TLSCOH WFSC.
     unfold issuable, issued. rewrite id_inter, <- !seqA. 
     eapply dom_rel_iord_ext_parts.
     3: by apply init_issued.
@@ -393,25 +401,25 @@ Definition issuable T :=
 
   Lemma ar_rfrmw_ct_issuable_in_I  :
     dom_rel (⦗W⦘ ⨾ (ar ∪ rf ⨾ rmw)⁺ ⨾ ⦗issuable T⦘) ⊆₁ issued T.
-  Proof using WF TLSCOH IMMCON.
+  Proof using WF TLSCOH WFSC.
     rewrite (rmw_in_ppo_loc WF). apply ar_rf_ppo_loc_ct_issuable_in_I.
   Qed.
 
   Lemma ar_rf_ppo_loc_ct_I_in_I  :
     dom_rel (⦗W⦘ ⨾ (ar ∪ rf ⨾ (ppo ∩ same_loc))⁺ ⨾ ⦗issued T⦘) ⊆₁ issued T.
-  Proof using WF TLSCOH IORDCOH IMMCON.
+  Proof using WF TLSCOH IORDCOH WFSC.
     rewrite issued_in_issuable at 1. apply ar_rf_ppo_loc_ct_issuable_in_I.
   Qed.
 
   Lemma ar_rfrmw_ct_I_in_I  :
     dom_rel (⦗W⦘ ⨾ (ar ∪ rf ⨾ rmw)⁺ ⨾ ⦗issued T⦘) ⊆₁ issued T.
-  Proof using WF TLSCOH IORDCOH IMMCON.
+  Proof using WF TLSCOH IORDCOH WFSC.
     rewrite issued_in_issuable at 1. apply ar_rfrmw_ct_issuable_in_I. 
   Qed.
 
   Lemma ar_rf_ppo_loc_rt_I_in_I  :
     dom_rel (⦗W⦘ ⨾ (ar ∪ rf ⨾ (ppo ∩ same_loc))＊ ⨾ ⦗issued T⦘) ⊆₁ issued T.
-  Proof using WF TLSCOH IORDCOH IMMCON.
+  Proof using WF TLSCOH IORDCOH WFSC.
     rewrite rtE. rewrite !seq_union_l, !seq_union_r, dom_union; unionL.
     { basic_solver. }
     apply ar_rf_ppo_loc_ct_I_in_I.
@@ -419,63 +427,63 @@ Definition issuable T :=
 
   Lemma ar_rfrmw_rt_I_in_I  :
     dom_rel (⦗W⦘ ⨾ (ar ∪ rf ⨾ rmw)＊ ⨾ ⦗issued T⦘) ⊆₁ issued T.
-  Proof using WF TLSCOH IORDCOH IMMCON.
+  Proof using WF TLSCOH IORDCOH WFSC.
     rewrite (rmw_in_ppo_loc WF). by apply ar_rf_ppo_loc_rt_I_in_I.
   Qed.
 
   Lemma ar_rf_ppo_loc_issuable_in_I:
     dom_rel (⦗W⦘ ⨾ (ar ∪ rf ⨾ (ppo ∩ same_loc)) ⨾ ⦗issuable T⦘) ⊆₁ issued T.
-  Proof using WF TLSCOH IMMCON. 
+  Proof using WF TLSCOH WFSC.
     rewrite ct_step with (r := ar ∪ rf ⨾ (ppo ∩ same_loc)).
     by apply ar_rf_ppo_loc_ct_issuable_in_I.
   Qed.     
 
   Lemma ar_rfrmw_issuable_in_I  :
     dom_rel (⦗W⦘ ⨾ (ar ∪ rf ⨾ rmw) ⨾ ⦗issuable T⦘) ⊆₁ issued T.
-  Proof using WF TLSCOH IMMCON.
+  Proof using WF TLSCOH WFSC.
     rewrite (rmw_in_ppo_loc WF). by apply ar_rf_ppo_loc_issuable_in_I.
   Qed.
 
   Lemma ar_rf_ppo_loc_I_in_I  :
     dom_rel (⦗W⦘ ⨾ (ar ∪ rf ⨾ (ppo ∩ same_loc)) ⨾ ⦗issued T⦘) ⊆₁ issued T.
-  Proof using WF TLSCOH IORDCOH IMMCON.
+  Proof using WF TLSCOH IORDCOH WFSC.
     rewrite ct_step with (r := ar ∪ rf ⨾ (ppo ∩ same_loc)).
     rewrite issued_in_issuable at 1. apply ar_rf_ppo_loc_ct_issuable_in_I.
   Qed.
 
   Lemma ar_rfrmw_I_in_I  :
     dom_rel (⦗W⦘ ⨾ (ar ∪ rf ⨾ rmw) ⨾ ⦗issued T⦘) ⊆₁ issued T.
-  Proof using WF TLSCOH IORDCOH IMMCON.
+  Proof using WF TLSCOH IORDCOH WFSC.
     rewrite (rmw_in_ppo_loc WF). by apply ar_rf_ppo_loc_I_in_I.
   Qed.
 
   Lemma ar_ct_issuable_in_I  :
     dom_rel (⦗W⦘ ⨾ ar⁺ ⨾ ⦗issuable T⦘) ⊆₁ issued T.
-  Proof using WF TLSCOH IMMCON. 
+  Proof using WF TLSCOH WFSC.
     arewrite (ar ⊆ ar ∪ rf ⨾ rmw). by apply ar_rfrmw_ct_issuable_in_I.
   Qed.
 
   Lemma ar_ct_I_in_I  :
     dom_rel (⦗W⦘ ⨾ ar⁺ ⨾ ⦗issued T⦘) ⊆₁ issued T.
-  Proof using WF TLSCOH IORDCOH IMMCON.
+  Proof using WF TLSCOH IORDCOH WFSC.
     rewrite issued_in_issuable at 1. apply ar_ct_issuable_in_I. 
   Qed.
 
   Lemma ar_issuable_in_I  :
     dom_rel (⦗W⦘ ⨾ ar ⨾ ⦗issuable T⦘) ⊆₁ issued T.
-  Proof using WF TLSCOH IMMCON.
+  Proof using WF TLSCOH WFSC.
     rewrite ct_step with (r:=ar). by apply ar_ct_issuable_in_I.
   Qed.
 
   Lemma ar_I_in_I  :
     dom_rel (⦗W⦘ ⨾ ar ⨾ ⦗issued T⦘) ⊆₁ issued T.
-  Proof using WF TLSCOH IORDCOH IMMCON.
+  Proof using WF TLSCOH IORDCOH WFSC.
     rewrite issued_in_issuable at 1. apply ar_issuable_in_I. 
   Qed.
 
   Lemma W_ar_coverable_in_I  :
     dom_rel (⦗W⦘ ⨾ ar ⨾ ⦗coverable T⦘) ⊆₁ issued T.
-  Proof using WF TLSCOH IORDCOH IMMCON.
+  Proof using WF TLSCOH IORDCOH WFSC.
     rewrite dom_eqv1. rewrite ar_coverable_in_CI.
     rewrite set_inter_union_r; unionL.
     2: basic_solver.
@@ -484,13 +492,13 @@ Definition issuable T :=
 
   Lemma W_ar_C_in_I  :
     dom_rel (⦗W⦘ ⨾ ar ⨾ ⦗covered T⦘) ⊆₁ issued T.
-  Proof using WF TLSCOH IORDCOH IMMCON. 
+  Proof using WF TLSCOH IORDCOH WFSC.
     rewrite covered_in_coverable. apply W_ar_coverable_in_I.
   Qed.
 
   Lemma W_ar_coverable_issuable_in_CI  :
     dom_rel (⦗W⦘ ⨾ ar ⨾ ⦗coverable T ∪₁ issuable T⦘) ⊆₁ issued T.
-  Proof using WF TLSCOH IORDCOH IMMCON.
+  Proof using WF TLSCOH IORDCOH WFSC.
     rewrite id_union, !seq_union_r, dom_union; unionL.
     { by apply W_ar_coverable_in_I. }
     apply ar_issuable_in_I.
@@ -499,7 +507,7 @@ Definition issuable T :=
 
   Lemma ar_rt_I_in_I  :
     dom_rel (⦗W⦘ ⨾ ar＊ ⨾ ⦗issued T⦘) ⊆₁ issued T.
-  Proof using WF TLSCOH IORDCOH IMMCON. 
+  Proof using WF TLSCOH IORDCOH WFSC.
     rewrite rtE, !seq_union_l, !seq_union_r, seq_id_l, dom_union.
     unionL; [basic_solver|]. by apply ar_ct_I_in_I.
   Qed.
@@ -535,92 +543,108 @@ Definition issuable T :=
     unfold RF. hahn_frame. basic_solver 10. 
   Qed.
 
-  Lemma rf_ppo_loc_coverable_in_I  :
+  Lemma rf_ppo_loc_issuable_in_I:
+    dom_rel (rf ⨾ ppo ∩ same_loc ⨾ ⦗issuable T⦘) ⊆₁ issued T.
+  Proof using WF TLSCOH.
+    unfold issuable. rewrite id_inter. 
+    rewrite <- !seqA. eapply dom_rel_iord_ext_parts.
+    3: { by rewrite init_issued. }
+    2: { rewrite wf_rfE, ppo_in_sb, wf_sbE, no_sb_to_init; basic_solver. }
+    erewrite eqv_rel_mori with (x := _ ∩₁ _); [| intro; apply proj2].
+    transitivity (AR G sc); [| unfold iord_simpl; basic_solver].
+    unfold AR. hahn_frame.
+    apply map_rel_mori; [done| ]. hahn_frame.
+    rewrite <- ct_step. rewrite (dom_l (wf_rfD WF)) at 1. basic_solver 10.
+  Qed. 
+
+  Lemma rf_ppo_loc_coverable_in_I:
     dom_rel (rf ⨾ (ppo ∩ same_loc) ⨾ ⦗coverable T⦘) ⊆₁ issued T.
-  Proof using WF TLSCOH IORDCOH IMMCON. 
-    arewrite (ppo ∩ same_loc ⊆ ppo).
-    rewrite (dom_l (wf_rfD WF)), seqA.
-    rewrite rfi_union_rfe, !seq_union_l, !seq_union_r, dom_union.
+  Proof using WF TLSCOH IORDCOH.
+    rewrite rfi_union_rfe, !seq_union_l, dom_union.
     unionL.
-    2: { rewrite (dom_r (@wf_ppoD G)), !seqA.
-         rewrite <- id_inter.
-         rewrite w_coverable_issued.
-         sin_rewrite rfe_ppo_in_ar_ct; auto.
-           by apply ar_ct_I_in_I. }
-    arewrite (rfi ⊆ sb).
-    rewrite (ppo_in_sb WF). sin_rewrite sb_sb.
-    rewrite dom_W_sb_coverable_in_I; auto.
+    2: { rewrite (dom_r (@wf_ppoD G)), seq_eqv_inter_lr, !seqA.
+         rewrite <- id_inter. rewrite w_coverable_issued.
+         rewrite issued_in_issuable at 1. rewrite rfe_in_rf. 
+         eapply rf_ppo_loc_issuable_in_I. }
+    rewrite (dom_l (wf_rfiD WF)), seqA.
+    rewrite inclusion_inter_l1. rewrite (ppo_in_sb WF), rfi_in_sb.
+    sin_rewrite sb_sb. rewrite dom_W_sb_coverable_in_I; auto.
   Qed.
 
   Lemma rfrmw_coverable_in_I  :
     dom_rel (rf ⨾ rmw ⨾ ⦗coverable T⦘) ⊆₁ issued T.
-  Proof using WF TLSCOH IORDCOH IMMCON. 
+  Proof using WF TLSCOH IORDCOH . 
     rewrite (rmw_in_ppo_loc WF). by apply rf_ppo_loc_coverable_in_I.
   Qed.
 
   Lemma rf_ppo_loc_C_in_I  :
     dom_rel (rf ⨾ (ppo ∩ same_loc) ⨾ ⦗covered T⦘) ⊆₁ issued T.
-  Proof using WF TLSCOH IORDCOH IMMCON.
+  Proof using WF TLSCOH IORDCOH .
     rewrite covered_in_coverable. apply rf_ppo_loc_coverable_in_I.
   Qed.
 
   Lemma rfrmw_C_in_I  :
     dom_rel (rf ⨾ rmw ⨾ ⦗covered T⦘) ⊆₁ issued T.
-  Proof using WF TLSCOH IORDCOH IMMCON.
+  Proof using WF TLSCOH IORDCOH .
     rewrite covered_in_coverable. apply rfrmw_coverable_in_I.
   Qed.
 
   Lemma rf_ppo_loc_coverable_issuable_in_I  :
     dom_rel (rf ⨾ (ppo ∩ same_loc) ⨾ ⦗coverable T ∪₁ issuable T⦘) ⊆₁ issued T.
-  Proof using WF TLSCOH IORDCOH IMMCON.
+  Proof using WF TLSCOH IORDCOH .
     rewrite id_union, !seq_union_r, dom_union.
     unionL.
     { apply rf_ppo_loc_coverable_in_I. }
-    rewrite (dom_l (wf_rfD WF)), !seqA.
-    arewrite (rf ⨾ ppo ∩ same_loc ⊆ ar ∪ rf ⨾ ppo ∩ same_loc).
-      by apply ar_rf_ppo_loc_issuable_in_I.
+    apply rf_ppo_loc_issuable_in_I. 
   Qed.
 
   Lemma rfrmw_coverable_issuable_in_I  :
     dom_rel (rf ⨾ rmw ⨾ ⦗coverable T ∪₁ issuable T⦘) ⊆₁ issued T.
-  Proof using WF TLSCOH IORDCOH IMMCON.
+  Proof using WF TLSCOH IORDCOH .
     rewrite (rmw_in_ppo_loc WF). by apply rf_ppo_loc_coverable_issuable_in_I.
   Qed.
 
   Lemma rf_ppo_loc_I_in_I  :
     dom_rel (rf ⨾ (ppo ∩ same_loc) ⨾ ⦗issued T⦘) ⊆₁ issued T.
-  Proof using WF TLSCOH IORDCOH IMMCON.
-    rewrite (dom_l (wf_rfD WF)), seqA.
-    arewrite (rf ⨾ (ppo ∩ same_loc) ⊆ ar ∪ rf ⨾ (ppo ∩ same_loc)).
-    by apply ar_rf_ppo_loc_I_in_I.
+  Proof using WF TLSCOH IORDCOH .
+    rewrite issued_in_issuable at 1. apply rf_ppo_loc_issuable_in_I. 
   Qed.
 
   Lemma rfrmw_I_in_I  :
     dom_rel (rf ⨾ rmw ⨾ ⦗issued T⦘) ⊆₁ issued T.
-  Proof using WF TLSCOH IORDCOH IMMCON.
+  Proof using WF TLSCOH IORDCOH .
     rewrite (rmw_in_ppo_loc WF). by apply rf_ppo_loc_I_in_I.
+  Qed.
+
+  (*TODO: move to lib*)
+  Lemma dom_rel_clos_refl_trans_eqv {A: Type} (r: relation A) (d: A -> Prop)
+        (DOM: dom_rel (r ⨾ ⦗d⦘) ⊆₁ d):
+    dom_rel (r^* ⨾ ⦗d⦘) ⊆₁ d. 
+  Proof using. 
+    rewrite rtEE. rewrite seq_bunion_l, dom_rel_bunion.
+    apply set_subset_bunion_l. intros n _. induction n.
+    { rewrite pow_0. basic_solver. }
+    rewrite pow_S_begin, seqA.
+    apply dom_rel_helper in IHn. rewrite IHn.
+    rewrite <- !seqA. do 2 rewrite dom_seq. auto. 
   Qed.
 
   Lemma rf_ppo_loc_rt_I_in_I  :
     dom_rel ((rf ⨾ ppo ∩ same_loc)＊ ⨾ ⦗issued T⦘) ⊆₁ issued T.
-  Proof using WF TLSCOH IORDCOH IMMCON.
-    rewrite rtE. rewrite !seq_union_l, !seq_id_l. rewrite dom_union.
-    unionL; [basic_solver|].
-    rewrite (dom_l (wf_rfD WF)). rewrite !seqA.
-    rewrite inclusion_ct_seq_eqv_l. rewrite !seqA.
-    arewrite (rf ⨾ ppo ∩ same_loc ⊆ ar ∪ rf ⨾ ppo ∩ same_loc).
-    apply ar_rf_ppo_loc_ct_I_in_I.
+  Proof using WF TLSCOH IORDCOH .
+    apply dom_rel_clos_refl_trans_eqv.
+    rewrite seqA. apply rf_ppo_loc_I_in_I. 
   Qed.
 
   Lemma rfrmw_rt_I_in_I  :
     dom_rel ((rf ⨾ rmw)＊ ⨾ ⦗issued T⦘) ⊆₁ issued T.
-  Proof using WF TLSCOH IORDCOH IMMCON.
+  Proof using WF TLSCOH IORDCOH .
     rewrite (rmw_in_ppo_loc WF). by apply rf_ppo_loc_rt_I_in_I.
   Qed.
 
   Lemma rf_ppo_loc_CI_in_I  :
     dom_rel (rf ⨾ (ppo ∩ same_loc) ⨾ ⦗covered T ∪₁ issued T⦘) ⊆₁ issued T.
-  Proof using WF TLSCOH IORDCOH IMMCON.
+  Proof using WF TLSCOH IORDCOH .
     rewrite id_union, !seq_union_r, dom_union.
     unionL.
     { by apply rf_ppo_loc_C_in_I. }
@@ -629,13 +653,13 @@ Definition issuable T :=
 
   Lemma rfrmw_CI_in_I  :
     dom_rel (rf ⨾ rmw ⨾ ⦗covered T ∪₁ issued T⦘) ⊆₁ issued T.
-  Proof using WF TLSCOH IORDCOH IMMCON.
+  Proof using WF TLSCOH IORDCOH .
     rewrite (rmw_in_ppo_loc WF). by apply rf_ppo_loc_CI_in_I.
   Qed.
 
   Lemma ar_rf_ppo_loc_coverable_in_CI  :
     dom_rel ((ar ∪ rf ⨾ ppo ∩ same_loc) ⨾ ⦗coverable T⦘) ⊆₁ covered T ∪₁ issued T.
-  Proof using WF IMMCON TLSCOH IORDCOH.
+  Proof using WF WFSC TLSCOH IORDCOH.
     rewrite seq_union_l, dom_union, !seqA.
     unionL.
     { by apply ar_coverable_in_CI. }
@@ -644,26 +668,26 @@ Definition issuable T :=
 
   Lemma ar_rfrmw_coverable_in_CI  :
     dom_rel ((ar ∪ rf ⨾ rmw) ⨾ ⦗coverable T⦘) ⊆₁ covered T ∪₁ issued T.
-  Proof using WF IMMCON TLSCOH IORDCOH.
+  Proof using WF WFSC TLSCOH IORDCOH.
     rewrite (rmw_in_ppo_loc WF). by apply ar_rf_ppo_loc_coverable_in_CI.
   Qed.
 
   Lemma ar_rf_ppo_loc_C_in_CI  :
     dom_rel ((ar ∪ rf ⨾ ppo ∩ same_loc) ⨾ ⦗covered T⦘) ⊆₁ covered T ∪₁ issued T.
-  Proof using WF IMMCON TLSCOH IORDCOH.
+  Proof using WF WFSC TLSCOH IORDCOH.
     rewrite covered_in_coverable at 1.
     apply ar_rf_ppo_loc_coverable_in_CI.
   Qed.
 
   Lemma ar_rfrmw_C_in_CI  :
     dom_rel ((ar ∪ rf ⨾ rmw) ⨾ ⦗covered T⦘) ⊆₁ covered T ∪₁ issued T.
-  Proof using WF IMMCON TLSCOH IORDCOH.
+  Proof using WF WFSC TLSCOH IORDCOH.
     rewrite (rmw_in_ppo_loc WF). by apply ar_rf_ppo_loc_C_in_CI.
   Qed.
 
   Lemma ar_rf_ppo_loc_coverable_issuable_in_I  :
     dom_rel (⦗W⦘ ⨾ (ar ∪ rf ⨾ ppo ∩ same_loc) ⨾ ⦗coverable T ∪₁ issuable T⦘) ⊆₁ issued T.
-  Proof using WF IMMCON TLSCOH IORDCOH.
+  Proof using WF WFSC TLSCOH IORDCOH.
     rewrite seq_union_l, seq_union_r, dom_union; unionL.
     { apply W_ar_coverable_issuable_in_CI. }
     arewrite_id ⦗W⦘. rewrite seq_id_l.
@@ -672,13 +696,13 @@ Definition issuable T :=
 
   Lemma ar_rfrmw_coverable_issuable_in_I  :
     dom_rel (⦗W⦘ ⨾ (ar ∪ rf ⨾ rmw) ⨾ ⦗coverable T ∪₁ issuable T⦘) ⊆₁ issued T.
-  Proof using WF IMMCON TLSCOH IORDCOH.
+  Proof using WF WFSC TLSCOH IORDCOH.
     rewrite (rmw_in_ppo_loc WF). by apply ar_rf_ppo_loc_coverable_issuable_in_I.
   Qed.
 
   Lemma ar_CI_in_CI  :
     dom_rel (⦗W⦘ ⨾ ar ⨾ ⦗covered T ∪₁ issued T⦘) ⊆₁ issued T.
-  Proof using WF TLSCOH IORDCOH IMMCON. 
+  Proof using WF WFSC TLSCOH IORDCOH . 
     rewrite id_union, !seq_union_r, dom_union; unionL.
     { by apply W_ar_C_in_I. }
     apply ar_I_in_I.
@@ -686,7 +710,7 @@ Definition issuable T :=
 
   Lemma ar_rf_ppo_loc_CI_in_I  :
     dom_rel (⦗W⦘ ⨾ (ar ∪ rf ⨾ ppo ∩ same_loc) ⨾ ⦗covered T ∪₁ issued T⦘) ⊆₁ issued T.
-  Proof using WF IMMCON TLSCOH IORDCOH.
+  Proof using WF WFSC TLSCOH IORDCOH.
     rewrite seq_union_l, seq_union_r, dom_union; unionL.
     { apply ar_CI_in_CI. }
     arewrite_id ⦗W⦘. rewrite seq_id_l.
@@ -695,13 +719,13 @@ Definition issuable T :=
 
   Lemma ar_rfrmw_CI_in_I  :
     dom_rel (⦗W⦘ ⨾ (ar ∪ rf ⨾ rmw) ⨾ ⦗covered T ∪₁ issued T⦘) ⊆₁ issued T.
-  Proof using WF IMMCON TLSCOH IORDCOH.
+  Proof using WF WFSC TLSCOH IORDCOH.
     rewrite (rmw_in_ppo_loc WF). by apply ar_rf_ppo_loc_CI_in_I.
   Qed.
 
   Lemma ar_rf_ppo_loc_ct_coverable_issuable_in_I  :
     dom_rel (⦗W⦘ ⨾ (ar ∪ rf ⨾ ppo ∩ same_loc)⁺ ⨾ ⦗coverable T ∪₁ issuable T⦘) ⊆₁ issued T.
-  Proof using WF IMMCON TLSCOH IORDCOH.
+  Proof using WF WFSC TLSCOH IORDCOH.
     intros x [y HH].
     destruct_seq HH as [AA BB].
     apply clos_trans_tn1 in HH.
@@ -733,13 +757,13 @@ Definition issuable T :=
 
   Lemma ar_rfrmw_ct_coverable_issuable_in_I  :
     dom_rel (⦗W⦘ ⨾ (ar ∪ rf ⨾ rmw)⁺ ⨾ ⦗coverable T ∪₁ issuable T⦘) ⊆₁ issued T.
-  Proof using WF IMMCON TLSCOH IORDCOH.
+  Proof using WF WFSC TLSCOH IORDCOH.
     rewrite (rmw_in_ppo_loc WF). apply ar_rf_ppo_loc_ct_coverable_issuable_in_I.
   Qed.
 
   Lemma ar_rf_ppo_loc_ct_CI_in_I  :
     dom_rel (⦗W⦘ ⨾ (ar ∪ rf ⨾ ppo ∩ same_loc)⁺ ⨾ ⦗covered T ∪₁ issued T⦘) ⊆₁ issued T.
-  Proof using WF IMMCON TLSCOH IORDCOH.
+  Proof using WF WFSC TLSCOH IORDCOH.
     rewrite covered_in_coverable.
     rewrite issued_in_issuable at 1.
     apply ar_rf_ppo_loc_ct_coverable_issuable_in_I.
@@ -747,13 +771,13 @@ Definition issuable T :=
 
   Lemma ar_rfrmw_ct_CI_in_I  :
     dom_rel (⦗W⦘ ⨾ (ar ∪ rf ⨾ rmw)⁺ ⨾ ⦗covered T ∪₁ issued T⦘) ⊆₁ issued T.
-  Proof using WF IMMCON TLSCOH IORDCOH.
+  Proof using WF WFSC TLSCOH IORDCOH.
     rewrite (rmw_in_ppo_loc WF). apply ar_rf_ppo_loc_ct_CI_in_I.
   Qed.
 
   Lemma ar_rf_ppo_loc_rt_coverable_in_I  :
     dom_rel (⦗W⦘ ⨾ (ar ∪ rf ⨾ ppo ∩ same_loc)＊ ⨾ ⦗coverable T⦘) ⊆₁ issued T.
-  Proof using WF IMMCON TLSCOH IORDCOH.
+  Proof using WF WFSC TLSCOH IORDCOH.
     rewrite rtE. rewrite !seq_union_l, !seq_union_r, dom_union, seq_id_l.
     unionL.
     { generalize w_coverable_issued. basic_solver. }
@@ -763,13 +787,13 @@ Definition issuable T :=
 
   Lemma ar_rfrmw_rt_coverable_in_I  :
     dom_rel (⦗W⦘ ⨾ (ar ∪ rf ⨾ rmw)＊ ⨾ ⦗coverable T⦘) ⊆₁ issued T.
-  Proof using WF IMMCON TLSCOH IORDCOH.
+  Proof using WF WFSC TLSCOH IORDCOH.
     rewrite (rmw_in_ppo_loc WF). apply ar_rf_ppo_loc_rt_coverable_in_I.
   Qed.
 
   Lemma ar_rf_ppo_loc_rt_CI_in_I  :
     dom_rel (⦗W⦘ ⨾ (ar ∪ rf ⨾ ppo ∩ same_loc)＊ ⨾ ⦗covered T ∪₁ issued T⦘) ⊆₁ issued T.
-  Proof using WF IMMCON TLSCOH IORDCOH.
+  Proof using WF WFSC TLSCOH IORDCOH.
     rewrite rtE. rewrite !seq_union_l, !seq_union_r, dom_union, seq_id_l.
     unionL.
     { generalize w_covered_issued. basic_solver. }
@@ -778,13 +802,13 @@ Definition issuable T :=
 
   Lemma ar_rfrmw_rt_CI_in_I  :
     dom_rel (⦗W⦘ ⨾ (ar ∪ rf ⨾ rmw)＊ ⨾ ⦗covered T ∪₁ issued T⦘) ⊆₁ issued T.
-  Proof using WF IMMCON TLSCOH IORDCOH.
+  Proof using WF WFSC TLSCOH IORDCOH.
     rewrite (rmw_in_ppo_loc WF). apply ar_rf_ppo_loc_rt_CI_in_I.
   Qed.
   
   Lemma ar_rt_C_in_I  :
     dom_rel (⦗W⦘ ⨾ ar＊ ⨾ ⦗covered T⦘) ⊆₁ issued T.
-  Proof using WF IMMCON TLSCOH IORDCOH.
+  Proof using WF WFSC TLSCOH IORDCOH.
     unfolder.
     ins. desf.
     apply clos_rt_rtn1 in H0.
@@ -805,7 +829,7 @@ Definition issuable T :=
 
   Lemma ar_rt_CI_in_I  :
     dom_rel (⦗W⦘ ⨾ ar＊ ⨾ ⦗covered T ∪₁ issued T⦘) ⊆₁ issued T.
-  Proof using WF IMMCON TLSCOH IORDCOH.
+  Proof using WF WFSC TLSCOH IORDCOH.
     rewrite id_union, !seq_union_r, dom_union; unionL.
     { by apply ar_rt_C_in_I. }
       by apply ar_rt_I_in_I.
@@ -814,128 +838,222 @@ Definition issuable T :=
   Lemma sbCsbI_CsbI   :
     sb ⨾ ⦗covered T ∪₁ dom_rel (sb^? ⨾ ⦗issued T⦘)⦘ ⊆
     ⦗covered T ∪₁ dom_rel (sb^? ⨾ ⦗issued T⦘)⦘ ⨾ sb.
-  Proof using WF TLSCOH IORDCOH IMMCON.
+  Proof using WF TLSCOH IORDCOH.
     rewrite id_union, !seq_union_r, !seq_union_l.
     apply union_mori.
     { rewrite sb_covered; eauto. basic_solver. }
     generalize (@sb_trans G). basic_solver 10.
   Qed.
 
+  Lemma dom_rfe_ppo_issuable_in_I :
+    dom_rel (rfe ⨾ ppo ⨾ ⦗issuable T⦘) ⊆₁ issued T.
+  Proof using WF TLSCOH.
+    unfold issuable. rewrite id_inter. rewrite <- !seqA.
+    apply dom_rel_iord_ext_parts.
+    3: { rewrite init_issued. basic_solver. }
+    2: { rewrite wf_rfeE, ppo_in_sb, wf_sbE, no_sb_to_init; basic_solver. }
+    transitivity (AR G sc); [| unfold iord_simpl; basic_solver 10].
+    erewrite eqv_rel_mori with (x := _ ∩₁ _); [| intro; apply proj2].
+    unfold AR. hahn_frame. apply map_rel_mori; [done| ].
+    rewrite (dom_l (wf_rfeD WF)). hahn_frame.
+    rewrite <- ct_unit, <- ct_step. unfold ar, ar_int.
+    apply seq_mori; basic_solver 10.
+  Qed.
+
   Lemma dom_rfe_ppo_issued :
     dom_rel (rfe ⨾ ppo ⨾ ⦗issued T⦘) ⊆₁ issued T.
-  Proof using WF TLSCOH IORDCOH IMMCON.
-    rewrite (dom_l (wf_rfeD WF)).
-    arewrite (rfe ⊆ ar).
-    rewrite ppo_in_ar.
-    sin_rewrite ar_ar_in_ar_ct.
-      by apply ar_ct_I_in_I.
+  Proof using WF TLSCOH IORDCOH.
+    rewrite issued_in_issuable at 1. apply dom_rfe_ppo_issuable_in_I. 
+  Qed.
+
+  Lemma dom_detour_ppo_issuable_in_I :
+    dom_rel (detour ⨾ ppo ⨾ ⦗issuable T⦘) ⊆₁ issued T.
+  Proof using WF TLSCOH.
+    unfold issuable. rewrite id_inter. rewrite <- !seqA.
+    apply dom_rel_iord_ext_parts.
+    3: { rewrite init_issued. basic_solver. }
+    2: { rewrite detour_in_sb, ppo_in_sb, wf_sbE, no_sb_to_init; basic_solver. }
+    transitivity (AR G sc); [| unfold iord_simpl; basic_solver 10].
+    erewrite eqv_rel_mori with (x := _ ∩₁ _); [| intro; apply proj2].
+    unfold AR. hahn_frame. apply map_rel_mori; [done| ].
+    rewrite (dom_l (wf_detourD WF)). hahn_frame.
+    rewrite <- ct_unit, <- ct_step. unfold ar, ar_int.
+    apply seq_mori; basic_solver 10.
   Qed.
 
   Lemma dom_detour_rfe_ppo_issuable :
     dom_rel ((detour ∪ rfe) ⨾ ppo ⨾ ⦗issuable T⦘) ⊆₁ issued T.
-  Proof using WF TLSCOH IMMCON.
-    rewrite (dom_l (wf_rfeD WF)).
-    rewrite (dom_l (wf_detourD WF)).
-    arewrite (rfe ⊆ ar).
-    arewrite (detour ⊆ ar).
-    relsf.
-    rewrite ppo_in_ar, !seqA.
-    sin_rewrite ar_ar_in_ar_ct.
-    apply ar_ct_issuable_in_I. 
+  Proof using WF TLSCOH.
+    repeat case_union _ _. rewrite dom_union.
+    rewrite dom_rfe_ppo_issuable_in_I, dom_detour_ppo_issuable_in_I. basic_solver.
   Qed.
   
   Lemma dom_detour_rfe_ppo_issued :
     dom_rel ((detour ∪ rfe) ⨾ ppo ⨾ ⦗issued T⦘) ⊆₁ issued T.
-  Proof using WF TLSCOH IORDCOH IMMCON.
+  Proof using WF TLSCOH IORDCOH.
     rewrite issued_in_issuable at 1.
     apply dom_detour_rfe_ppo_issuable.
   Qed.
 
+  (* Lemma R_acq_sb_issuable_in_I: *)
+  (*   dom_rel (⦗R ∩₁ Acq⦘ ⨾ sb ⨾ ⦗issuable T⦘) ⊆₁ issued T. *)
+  (* Proof using. *)
+  (*   unfold issuable. rewrite id_inter with (s := _ ∩₁ _). rewrite <- !seqA. *)
+  (*   apply dom_rel_iord_ext_parts. *)
+  (*   3: { rewrite init_issued. basic_solver. } *)
+  (*   2: { rewrite wf_sbE, no_sb_to_init; basic_solver. } *)
+  (*   transitivity (AR G sc); [| unfold iord_simpl; basic_solver 10]. *)
+  (*   erewrite eqv_rel_mori with (x := _ ∩₁ W); [| intro; apply proj2]. *)
+  (*   unfold AR. hahn_frame. apply map_rel_mori; [done| ]. *)
+  (*   hahn_frame. rewrite <- ct_step. unfold ar, ar_int. *)
+  (*   apply seq_mori; basic_solver 10. *)
+
   Lemma dom_detour_rfe_acq_sb_issuable :
     dom_rel ((detour ∪ rfe) ⨾ ⦗R ∩₁ Acq⦘ ⨾ sb ⨾ ⦗issuable T⦘) ⊆₁ issued T.
-  Proof using WF TLSCOH IMMCON.
-    rewrite (dom_l (wf_detourD WF)).
-    rewrite (dom_l (wf_rfeD WF)).
-    arewrite (rfe ⊆ ar).
-    arewrite (detour ⊆ ar).
-    relsf.
-    arewrite (⦗R ∩₁ Acq⦘ ⨾ sb ⊆ ar).
-    { arewrite (⦗R ∩₁ Acq⦘ ⨾ sb ⊆ bob). unfold imm_s.ar, ar_int. eauto with hahn. }
-    sin_rewrite ar_ar_in_ar_ct.
-    apply ar_ct_issuable_in_I. 
+  Proof using WF TLSCOH.
+    unfold issuable. rewrite id_inter with (s := _ ∩₁ _). rewrite <- !seqA.
+    apply dom_rel_iord_ext_parts.
+    3: { rewrite init_issued. basic_solver. }
+    2: { rewrite detour_in_sb, wf_sbE, wf_rfeE, no_sb_to_init; basic_solver. }
+    transitivity (AR G sc); [| unfold iord_simpl; basic_solver 10].
+    erewrite eqv_rel_mori with (x := _ ∩₁ W); [| intro; apply proj2].
+    unfold AR. hahn_frame. apply map_rel_mori; [done| ].
+    rewrite (dom_l (wf_detourD WF)), (dom_l (wf_rfeD WF)), <- seq_union_r.
+    hahn_frame. rewrite <- ct_unit, <- ct_step.
+    unfold ar, ar_int, bob. apply seq_mori; basic_solver 10.
   Qed.
 
   Lemma dom_detour_rfe_acq_sb_issued :
     dom_rel ((detour ∪ rfe) ⨾ ⦗R ∩₁ Acq⦘ ⨾ sb ⨾ ⦗issued T⦘) ⊆₁ issued T.
-  Proof using WF TLSCOH IORDCOH IMMCON.
+  Proof using WF TLSCOH IORDCOH. 
     rewrite issued_in_issuable at 1.
     apply dom_detour_rfe_acq_sb_issuable.
   Qed.
 
+  Lemma rfe_ar_int_issuable_in_I  :
+    dom_rel (⦗W⦘ ⨾ (rfe ∪ ar_int G) ⨾ ⦗issuable T⦘) ⊆₁ issued T.
+  Proof using WF TLSCOH.
+    unfold issuable. rewrite id_inter with (s := _ ∩₁ _). rewrite <- !seqA.
+    apply dom_rel_iord_ext_parts.
+    3: { rewrite init_issued. basic_solver. }
+    2: { rewrite rfe_in_rf, wf_rfE, ar_int_in_sb, wf_sbE, no_sb_to_init, no_rf_to_init; basic_solver 10. }
+    transitivity (AR G sc); [| unfold iord_simpl; basic_solver 10].
+    unfold AR. hahn_frame.
+    erewrite eqv_rel_mori with (x := _ ∩₁ W); [| intro; apply proj2].
+    apply map_rel_mori; [done|]. hahn_frame.
+    rewrite <- ct_step. unfold ar. basic_solver. 
+  Qed. 
+
+  Lemma dom_detour_rfe_rmw_rfi_rmw_rt_I_in_I:
+    dom_rel ((((detour ∪ rfe) ⨾ (rmw ⨾ rfi)＊) ⨾ rmw) ⨾ ⦗issued T⦘) ⊆₁ issued T.
+  Proof using WF TLSCOH IORDCOH. 
+    rewrite !seqA. seq_rewrite rt_seq_swap. rewrite seqA.
+    assert (dom_rel ((rfi ⨾ rmw)＊ ⨾ ⦗issued T⦘) ⊆₁ (issued T)) as D2.
+    { apply dom_rel_clos_refl_trans_eqv.
+      rewrite <- rfrmw_CI_in_I at 2. rewrite rfi_in_rf. basic_solver 10. }
+    apply dom_rel_helper in D2. rewrite D2.
+    rewrite <- !seqA. do 2 rewrite dom_seq. rewrite seqA.
+
+    rewrite issued_in_issuable at 1.
+    unfold issuable. rewrite id_inter. rewrite <- !seqA. 
+    apply dom_rel_iord_ext_parts.
+    3: { rewrite init_issued. basic_solver. }
+    2: { rewrite rmw_in_sb, detour_in_sb, wf_rfeE, wf_sbE, no_sb_to_init; basic_solver. }
+    transitivity (AR G sc); [| unfold iord_simpl; basic_solver 10].
+    unfold AR. hahn_frame. apply map_rel_mori; [done| ].
+    rewrite (dom_l (wf_detourD WF)), (dom_l (wf_rfeD WF)), <- seq_union_r.
+    erewrite eqv_rel_mori with (x := _ ∩₁ W); [| intro; apply proj2].
+    hahn_frame. 
+    rewrite <- ct_unit, <- ct_step. unfold ar. apply seq_mori.
+    { unfold ar_int. basic_solver 10. }
+    rewrite rmw_in_ar_int; auto. basic_solver 10. 
+  Qed. 
+
   Lemma dom_detour_rmwrfi_rfe_acq_sb_issuable :
     dom_rel ((detour ∪ rfe) ⨾ (rmw ⨾ rfi)＊ ⨾ ⦗R ∩₁ Acq⦘ ⨾ sb ⨾ ⦗issuable T⦘) ⊆₁ issued T.
-  Proof using WF TLSCOH IMMCON.
-    arewrite (⦗R ∩₁ Acq⦘ ⊆ ⦗Acq⦘ ⨾ ⦗R ∩₁ Acq⦘) by basic_solver.
-    arewrite (rfi ⊆ rf).
-    sin_rewrite (@rmwrf_rt_Acq_in_ar_rfrmw_rt G WF sc); auto.
-    rewrite (dom_l (wf_detourD WF)).
-    rewrite (dom_l (wf_rfeD WF)).
-    arewrite (rfe ⊆ ar).
-    arewrite (detour ⊆ ar).
-    relsf.
-    arewrite (⦗R ∩₁ Acq⦘ ⨾ sb ⊆ ar).
-    { arewrite (⦗R ∩₁ Acq⦘ ⨾ sb ⊆ bob). unfold imm_s.ar, ar_int. eauto with hahn. }
-    arewrite (ar ⊆ ar ∪ rf ⨾ rmw) at 3.
-    arewrite (ar ⊆ ar ∪ rf ⨾ rmw) at 1.
-    seq_rewrite <- ct_end.
-    arewrite ((ar ∪ rf ⨾ rmw) ⨾ (ar ∪ rf ⨾ rmw)⁺ ⊆ (ar ∪ rf ⨾ rmw)⁺).
-    { rewrite ct_step with (r:= ar ∪ rf ⨾ rmw) at 1. apply ct_ct. }
-    apply ar_rfrmw_ct_issuable_in_I.
+  Proof using WF TLSCOH IORDCOH.
+    remember (detour ∪ rfe) as DR.
+    rewrite rtE. repeat case_union _ _. rewrite dom_union. subst DR.
+    apply set_subset_union_l. split.
+    { rewrite seq_id_l. apply dom_detour_rfe_acq_sb_issuable. }
+    rewrite ct_end. 
+    rewrite AuxRel2.r_to_r_codom_rel_r with (r := rmw) at 2. rewrite !seqA.
+
+    assert (dom_rel (⦗codom_rel rmw⦘ ⨾ rfi ⨾ ⦗R ∩₁ Acq⦘ ⨾ sb ⨾ ⦗issuable T⦘) ⊆₁ issued T) as D1.
+    { unfold issuable. rewrite id_inter with (s := _ ∩₁ _). rewrite <- !seqA.
+      apply dom_rel_iord_ext_parts.
+      3: { rewrite init_issued. basic_solver. }
+      2: { rewrite wf_rfiE, wf_sbE, no_sb_to_init; basic_solver. }
+      transitivity (AR G sc); [| unfold iord_simpl; basic_solver 10].
+      unfold AR. hahn_frame.
+      erewrite eqv_rel_mori with (x := _ ∩₁ W); [| intro; apply proj2].
+      apply map_rel_mori; [done|].
+      rewrite <- seq_eqvK with (dom := codom_rel rmw), !seqA.
+      arewrite (codom_rel rmw ⊆₁ W) at 1 by (rewrite wf_rmwD; basic_solver).
+      hahn_frame. 
+      rewrite <- seq_eqvK with (dom := R ∩₁ Acq), !seqA.
+      rewrite <- ct_unit. do 2 rewrite <- seqA. apply seq_mori.
+      { rewrite <- ct_step. unfold ar, ar_int. unfold W_ex. basic_solver 10. }
+      unfold ar, ar_int. unfold bob. basic_solver 10. }
+    apply dom_rel_helper in D1. rewrite D1.
+    rewrite <- !seqA. do 5 rewrite dom_seq.
+    apply dom_detour_rfe_rmw_rfi_rmw_rt_I_in_I. 
   Qed.
 
   Lemma dom_detour_rmwrfi_rfe_acq_sb_issued :
     dom_rel ((detour ∪ rfe) ⨾ (rmw ⨾ rfi)＊ ⨾ ⦗R ∩₁ Acq⦘ ⨾ sb ⨾ ⦗issued T⦘) ⊆₁ issued T.
-  Proof using WF TLSCOH IORDCOH IMMCON.
+  Proof using WF TLSCOH IORDCOH IORDCOH.
     rewrite issued_in_issuable at 1.
     apply dom_detour_rmwrfi_rfe_acq_sb_issuable.
   Qed.
 
   Lemma dom_rfe_acq_sb_issuable :
     dom_rel (rfe ⨾ ⦗R ∩₁ Acq⦘ ⨾ sb ⨾ ⦗issuable T⦘) ⊆₁ issued T.
-  Proof using WF TLSCOH IMMCON.
+  Proof using WF TLSCOH.
     arewrite (rfe ⊆ detour ∪ rfe).
     apply dom_detour_rfe_acq_sb_issuable.
   Qed.
 
   Lemma dom_rfe_acq_sb_issued :
     dom_rel (rfe ⨾ ⦗R ∩₁ Acq⦘ ⨾ sb ⨾ ⦗issued T⦘) ⊆₁ issued T.
-  Proof using WF TLSCOH IORDCOH IMMCON.
+  Proof using WF TLSCOH IORDCOH.
     rewrite issued_in_issuable at 1.
     apply dom_rfe_acq_sb_issuable.
   Qed.
 
+  Lemma W_ex_acq_sb_in_ar_int_W:
+    ⦗W_ex_acq⦘ ⨾ sb ⨾ ⦗W⦘ ⊆ ⦗W⦘ ⨾ ar_int G ⨾ ⦗W⦘. 
+  Proof using WF. 
+    rewrite <- seq_eqvK. rewrite <- seq_eqvK with (dom := W) at 1.
+    arewrite (W_ex_acq ⊆₁ W) at 1.
+    { unfold W_ex. rewrite wf_rmwD; basic_solver. }
+    hahn_frame. unfold ar_int. basic_solver 10.
+  Qed. 
+
   Lemma dom_wex_sb_issuable :
     dom_rel (⦗W_ex_acq⦘ ⨾ sb ⨾ ⦗issuable T⦘) ⊆₁ issued T.
-  Proof using WF TLSCOH IMMCON.
-    arewrite (⦗W_ex_acq⦘ ⊆ ⦗W⦘ ⨾ ⦗W_ex_acq⦘).
-    { rewrite <- seq_eqvK at 1.
-      rewrite (W_ex_in_W WF) at 1. basic_solver. }
-    arewrite (⦗issuable T⦘ ⊆ ⦗W⦘ ⨾ ⦗issuable T⦘).
-    { unfold issuable. basic_solver 10. }
-    arewrite (⦗W_ex_acq⦘ ⨾ sb ⨾ ⦗W⦘ ⊆ ar).
-    apply ar_issuable_in_I. 
+  Proof using WF TLSCOH.
+    unfold issuable. rewrite id_inter with (s := _ ∩₁ _). rewrite <- !seqA. 
+    apply dom_rel_iord_ext_parts.
+    3: { rewrite init_issued. basic_solver. }
+    2: { rewrite wf_sbE, no_sb_to_init; basic_solver. }
+    transitivity (AR G sc); [| unfold iord_simpl; basic_solver 10].
+    unfold AR. hahn_frame. apply map_rel_mori; [done| ].
+    erewrite eqv_rel_mori with (x := _ ∩₁ W); [| intro; apply proj2].
+    rewrite W_ex_acq_sb_in_ar_int_W. 
+    rewrite <- ct_step. unfold ar. basic_solver 10. 
   Qed.
 
   Lemma dom_wex_sb_issued :
     dom_rel (⦗W_ex_acq⦘ ⨾ sb ⨾ ⦗issued T⦘) ⊆₁ issued T.
-  Proof using WF TLSCOH IORDCOH IMMCON.
+  Proof using WF TLSCOH IORDCOH.
     rewrite issued_in_issuable at 1.
     apply dom_wex_sb_issuable.
   Qed.
   
   Lemma rf_rmw_issued_rfi_rmw_issued : 
     (rf ⨾ rmw)＊ ⨾ ⦗issued T⦘ ⊆ (rfi ⨾ rmw)＊ ⨾ ⦗issued T⦘ ⨾ (rf ⨾ rmw)＊.
-  Proof using WF IMMCON TLSCOH IORDCOH.
+  Proof using WF TLSCOH IORDCOH.
     assert (transitive sb) as SBT by apply sb_trans.
     eapply rt_ind_left with (P:= fun r => r ⨾ ⦗issued T⦘).
     { by eauto with hahn. }
@@ -949,17 +1067,9 @@ Definition issuable T :=
     arewrite (rfe ⨾ rmw ⨾ (rfi ⨾ rmw)＊ ⨾ ⦗issued T⦘ ⊆
                   ⦗issued T⦘ ⨾ rfe ⨾ rmw ⨾ (rfi ⨾ rmw)＊ ⨾ ⦗issued T⦘).
     { apply dom_rel_helper.
-      arewrite (rmw ⨾ (rfi ⨾ rmw)＊ ⊆ ar＊).
-      { arewrite (rfi ⊆ rf).
-        rewrite (rmw_in_ppo WF) at 1. rewrite ppo_in_ar.
-        rewrite rtE at 1. rewrite seq_union_r, seq_id_r.
-        apply inclusion_union_l.
-        { rewrite ct_step at 1. apply inclusion_t_rt. }
-        rewrite rmw_in_ppo_loc; auto.
-        rewrite ar_rf_ppo_loc_ct_in_ar_ct; auto. apply inclusion_t_rt. }
-      rewrite (dom_l (wf_rfeD WF)), !seqA.
-      arewrite (rfe ⊆ ar) at 1.
-      seq_rewrite <- ct_begin. by apply ar_ct_I_in_I. }
+      rewrite <- dom_detour_rfe_rmw_rfi_rmw_rt_I_in_I at 2. apply dom_rel_mori.
+      hahn_frame_r. rewrite <- rt_seq_swap. basic_solver 10. }
+
     arewrite (rfe ⨾ rmw ⊆ rf ⨾ rmw).
     arewrite (rfi ⊆ rf).
     arewrite (rf ⨾ rmw ⨾ (rf ⨾ rmw)＊ ⊆ (rf ⨾ rmw)⁺).
@@ -970,7 +1080,7 @@ Definition issuable T :=
   
   Lemma wex_rfi_rfe_rmw_issued_is_issued :
     dom_rel ((⦗ W_ex_acq ⦘ ⨾ rfi ∪ rfe) ⨾ rmw ⨾ ⦗ issued T ⦘) ⊆₁ issued T.
-  Proof using WF TLSCOH IORDCOH IMMCON.
+  Proof using WF TLSCOH IORDCOH.
     rewrite seq_union_l. rewrite dom_union.
     apply set_subset_union_l; split.
     { rewrite seqA. rewrite (rfi_in_sbloc' WF). rewrite (rmw_in_sb WF).
@@ -981,28 +1091,33 @@ Definition issuable T :=
       arewrite (⦗W_ex_acq⦘ ⊆ ⦗W⦘ ⨾ ⦗W_ex_acq⦘).
       { rewrite <- seq_eqvK at 1.
         rewrite (W_ex_in_W WF) at 1. basic_solver. }
-      arewrite (⦗W_ex_acq⦘ ⨾ sb ⨾ ⦗W⦘ ⊆ ar).
-      rewrite ct_step with (r:=ar).
-      apply ar_ct_I_in_I. }
+
+      rewrite issued_in_issuable at 1.
+      unfold issuable. rewrite id_inter with (s := _ ∩₁ _). rewrite <- !seqA.
+      apply dom_rel_iord_ext_parts.
+      3: { rewrite init_issued. basic_solver. }
+      2: { rewrite wf_sbE, no_sb_to_init; basic_solver. }
+      transitivity (AR G sc); [| unfold iord_simpl; basic_solver 10].
+      unfold AR. hahn_frame. apply map_rel_mori; [done|]. 
+      erewrite eqv_rel_mori with (x := _ ∩₁ W); [| intro; apply proj2].
+      sin_rewrite W_ex_acq_sb_in_ar_int_W.
+      unfold ar. rewrite <- ct_step. basic_solver 10. } 
+     
     rewrite (rmw_in_ppo WF).
-    rewrite ppo_in_ar.
-    rewrite (dom_l (wf_rfeD WF)), !seqA.
-    arewrite (rfe ⊆ ar).
-    sin_rewrite ar_ar_in_ar_ct.
-    apply ar_ct_I_in_I.
+    apply dom_rfe_ppo_issued. 
   Qed. 
 
   Lemma wex_rf_rmw_issued_is_issued :
     dom_rel (⦗ W_ex_acq ⦘ ⨾ rf ⨾ rmw ⨾ ⦗ issued T ⦘) ⊆₁ issued T.
-  Proof using WF TLSCOH IORDCOH IMMCON.
+  Proof using WF TLSCOH IORDCOH.
     arewrite (⦗W_ex_acq⦘ ⨾ rf ⊆ (⦗ W_ex_acq ⦘ ⨾ rfi ∪ rfe)).
     { rewrite rfi_union_rfe. basic_solver. }
-      by apply wex_rfi_rfe_rmw_issued_is_issued.
+    by apply wex_rfi_rfe_rmw_issued_is_issued.
   Qed.
 
   Lemma rf_rmw_issued :
     (rf ⨾ rmw)＊ ⨾ ⦗issued T⦘ ⊆ (rf ⨾ rmw ⨾ ⦗issued T⦘)＊.
-  Proof using WF TLSCOH IORDCOH IMMCON.
+  Proof using WF TLSCOH IORDCOH.
     intros x y HH. destruct_seq_r HH as II.
     apply clos_rt_rtn1 in HH.
     induction HH as [|y z TT].
@@ -1011,23 +1126,30 @@ Definition issuable T :=
     split.
     2: apply seqA; basic_solver.
     apply IHHH.
-    apply ar_rfrmw_I_in_I. exists z.
-    apply seq_eqv_lr. splits; auto.
-    2: by right.
-    red in TT. desf. apply (wf_rfD WF) in TT. unfolder in TT. desf.
+    apply rfrmw_I_in_I. exists z. apply seqA. basic_solver 10. 
   Qed.
+
+  Lemma fwbob_issuable_in_C:
+    dom_rel (fwbob ⨾ ⦗issuable T⦘) ⊆₁ covered T. 
+  Proof using TLSCOH.
+    unfold issuable. rewrite id_inter with (s := _ ∩₁ _). rewrite <- !seqA. 
+    apply dom_rel_iord_ext_parts.
+    3: { rewrite init_covered. basic_solver. }
+    2: { rewrite fwbob_in_sb, wf_sbE, no_sb_to_init; basic_solver. }
+    transitivity (FWBOB G); [| unfold iord_simpl; basic_solver 10].
+    unfold FWBOB. hahn_frame. basic_solver. 
+  Qed. 
 
   Lemma fwbob_I_in_C:
     dom_rel (fwbob ⨾ ⦗issued T⦘) ⊆₁ covered T. 
-  Proof using WF TLSCOH IORDCOH IMMCON.
-    arewrite (⦗issued T⦘ ⊆ ⦗W⦘ ⨾ ⦗issued T⦘) at 1.
-    { rewrite <- id_inter. apply eqv_rel_mori. split; auto using issuedW. }
-    rewrite <- seqA. apply dom_rel_iord_parts. unfold iord_simpl, FWBOB. intuition.
-  Qed.     
+  Proof using WF TLSCOH IORDCOH.
+    rewrite issued_in_issuable at 1.
+    apply fwbob_issuable_in_C. 
+  Qed.
 
   Lemma dom_W_Rel_sb_loc_I_in_C :
     dom_rel (⦗W ∩₁ Rel⦘ ⨾ sb ∩ same_loc ⨾ ⦗W⦘ ⨾ ⦗issued T⦘) ⊆₁ covered T.
-  Proof using WF TLSCOH IORDCOH IMMCON.
+  Proof using WF TLSCOH IORDCOH.
     arewrite (issued T ⊆₁ dom_cond fwbob (covered T)).
     { apply dom_rel_to_cond, fwbob_I_in_C. }
     rewrite <- !seqA.
@@ -1046,7 +1168,7 @@ Definition issuable T :=
   Lemma W_rel_sb_loc_W_CI :
     (⦗W ∩₁ Rel⦘ ⨾ sb ∩ same_loc ⨾ ⦗W⦘) ⨾ ⦗covered T ∪₁ issued T⦘ ⊆
     ⦗covered T ∪₁ issued T⦘ ⨾ (⦗W ∩₁ Rel⦘ ⨾ sb ∩ same_loc ⨾ ⦗W⦘).
-  Proof using WF TLSCOH IORDCOH IMMCON.
+  Proof using WF TLSCOH IORDCOH.
     (* case_refl _; [basic_solver|]. *)
     rewrite !seqA.
     arewrite (⦗W⦘ ⨾ ⦗covered T ∪₁ issued T⦘ ⊆ ⦗W⦘ ⨾ ⦗issued T⦘).
@@ -1058,54 +1180,54 @@ Definition issuable T :=
 
   Lemma sb_W_rel_CI :
     (sb ⨾ ⦗W ∩₁ Rel⦘) ⨾ ⦗covered T ∪₁ issued T⦘ ⊆ ⦗covered T ∪₁ issued T⦘ ⨾ (sb ⨾ ⦗W ∩₁ Rel⦘).
-  Proof using RELCOV WF TLSCOH IORDCOH IMMCON.
+  Proof using RELCOV WF TLSCOH IORDCOH.
     generalize RELCOV, dom_sb_covered.
     basic_solver 12.
   Qed.
 
   Lemma W_Rel_sb_loc_I : dom_rel (⦗W ∩₁ Rel⦘ ⨾  (sb ∩ same_loc) ⨾ ⦗W ∩₁ issued T⦘) ⊆₁ issued T.
-  Proof using WF TLSCOH IORDCOH IMMCON.
+  Proof using WF TLSCOH IORDCOH.
     generalize dom_W_Rel_sb_loc_I_in_C, w_covered_issued. basic_solver 21.
   Qed.
 
   Lemma sb_loc_issued  :
     ⦗W ∩₁ Rel⦘ ⨾ sb ∩ same_loc ⨾ ⦗W⦘ ⨾ ⦗issued T⦘ ⊆ 
                ⦗covered T⦘ ⨾ ⦗W ∩₁ Rel⦘ ⨾ sb ∩ same_loc ⨾ ⦗W⦘.
-  Proof using WF TLSCOH IORDCOH IMMCON.
+  Proof using WF TLSCOH IORDCOH.
     seq_rewrite (dom_rel_helper dom_W_Rel_sb_loc_I_in_C).
     basic_solver.
   Qed.
 
   Lemma dom_F_sb_I_in_C :
     dom_rel (⦗F ∩₁ Acq/Rel⦘ ⨾ sb ⨾ ⦗issued T⦘) ⊆₁ covered T.
-  Proof using WF TLSCOH IORDCOH IMMCON. 
+  Proof using WF TLSCOH IORDCOH. 
     arewrite (issued T ⊆₁ dom_cond fwbob (covered T)).
     { apply dom_rel_to_cond, fwbob_I_in_C. }
     rewrite <- !seqA.
     rewrite dom_cond_elim1; [basic_solver 21|].
     unfold imm_bob.fwbob.
     basic_solver 12.
-  Qed. 
+  Qed.
 
   Lemma F_sb_I_in_C  :
     ⦗F ∩₁ Acq/Rel⦘ ⨾ sb ⨾ ⦗issued T⦘ ⊆ ⦗covered T⦘ ⨾ ⦗F ∩₁ Acq/Rel⦘ ⨾ sb.
-  Proof using WF TLSCOH IORDCOH IMMCON. 
+  Proof using WF TLSCOH IORDCOH. 
     seq_rewrite (dom_rel_helper dom_F_sb_I_in_C). basic_solver.
   Qed.
 
   Lemma dom_F_Rel_sb_I_in_C :  dom_rel (⦗F ∩₁ Rel⦘ ⨾  sb ⨾ ⦗issued T⦘) ⊆₁ covered T.
-  Proof using RELCOV WF TLSCOH IORDCOH IMMCON.
+  Proof using RELCOV WF TLSCOH IORDCOH.
     etransitivity; [|apply dom_F_sb_I_in_C]; mode_solver 21.
   Qed.
 
   Lemma dom_F_Acq_sb_I_in_C :  dom_rel (⦗F ∩₁ Acq⦘ ⨾  sb ⨾ ⦗issued T⦘) ⊆₁ covered T.
-  Proof using RELCOV WF TLSCOH IORDCOH IMMCON. 
+  Proof using RELCOV WF TLSCOH IORDCOH. 
     etransitivity; [|apply dom_F_sb_I_in_C]; mode_solver 12. 
   Qed.
   
   Lemma dom_release_issued :
     dom_rel (release ⨾ ⦗ issued T ⦘) ⊆₁ covered T.
-  Proof using WF IMMCON RELCOV TLSCOH IORDCOH.
+  Proof using WF RELCOV TLSCOH IORDCOH.
     unfold imm_s_hb.release, imm_s_hb.rs.
     rewrite !seqA.
     sin_rewrite rf_rmw_issued_rfi_rmw_issued.
@@ -1124,14 +1246,14 @@ Definition issuable T :=
 
   Lemma release_issued :
     release ⨾ ⦗ issued T ⦘ ⊆ ⦗covered T⦘ ⨾ release.
-  Proof using WF RELCOV IMMCON TLSCOH IORDCOH.
+  Proof using WF RELCOV TLSCOH IORDCOH.
     seq_rewrite (dom_rel_helper dom_release_issued).
     basic_solver.
   Qed.
 
   Lemma dom_release_rf_covered :
     dom_rel (release ⨾ rf ⨾ ⦗ covered T ⦘) ⊆₁ covered T.
-  Proof using WF RELCOV IMMCON TLSCOH IORDCOH.
+  Proof using WF RELCOV TLSCOH IORDCOH.
     generalize dom_release_issued.
     generalize dom_rf_covered.
     basic_solver 21.
@@ -1139,14 +1261,14 @@ Definition issuable T :=
 
   Lemma release_rf_covered :
     release ⨾ rf ⨾ ⦗ covered T ⦘ ⊆ ⦗ covered T ⦘ ⨾ release ⨾ rf.
-  Proof using WF RELCOV IMMCON TLSCOH IORDCOH.
+  Proof using WF RELCOV TLSCOH IORDCOH.
     seq_rewrite (dom_rel_helper dom_release_rf_covered).
     basic_solver.
   Qed.
 
   Lemma dom_sb_W_rel_issued  :
     dom_rel (sb ⨾ ⦗W ∩₁ Rel⦘ ⨾ ⦗issued T⦘) ⊆₁ covered T.
-  Proof using WF TLSCOH IORDCOH IMMCON.
+  Proof using WF TLSCOH IORDCOH.
     arewrite (issued T ⊆₁ dom_cond fwbob (covered T)).
     { apply dom_rel_to_cond, fwbob_I_in_C. }
     rewrite <- !seqA.
@@ -1157,14 +1279,14 @@ Definition issuable T :=
 
   Lemma sb_W_rel_issued  :
     sb ⨾ ⦗W ∩₁ Rel⦘ ⨾ ⦗issued T⦘ ⊆ ⦗covered T⦘ ⨾ sb ⨾ ⦗W ∩₁ Rel⦘.
-  Proof using WF TLSCOH IORDCOH IMMCON.
+  Proof using WF TLSCOH IORDCOH.
     seq_rewrite (dom_rel_helper dom_sb_W_rel_issued).
     basic_solver.
   Qed.
 
   Lemma dom_sw_covered :
     dom_rel (sw ⨾ ⦗ covered T ⦘) ⊆₁ covered T.
-  Proof using WF RELCOV IMMCON TLSCOH IORDCOH.
+  Proof using WF RELCOV TLSCOH IORDCOH.
     unfold imm_s_hb.sw.
     generalize dom_sb_covered.
     generalize dom_release_rf_covered.
@@ -1172,14 +1294,14 @@ Definition issuable T :=
   Qed.
 
   Lemma sw_covered : sw ⨾ ⦗ covered T ⦘ ⊆ ⦗covered T⦘ ⨾ sw.
-  Proof using WF RELCOV IMMCON TLSCOH IORDCOH.
+  Proof using WF RELCOV TLSCOH IORDCOH.
     seq_rewrite (dom_rel_helper dom_sw_covered).
     basic_solver.
   Qed.
 
   Lemma hb_covered :
     hb ⨾ ⦗ covered T ⦘ ⊆ ⦗covered T⦘ ⨾ hb.
-  Proof using WF RELCOV IMMCON TLSCOH IORDCOH.
+  Proof using WF RELCOV TLSCOH IORDCOH.
     unfold imm_s_hb.hb.
     assert (A: (sb ∪ sw) ⨾ ⦗covered T⦘ ⊆ ⦗covered T⦘ ⨾ (sb ∪ sw)⁺).
     { relsf.
@@ -1195,13 +1317,13 @@ Definition issuable T :=
 
   Lemma dom_hb_covered :
     dom_rel (hb ⨾ ⦗ covered T ⦘) ⊆₁ covered T.
-  Proof using WF RELCOV IMMCON TLSCOH IORDCOH.
+  Proof using WF RELCOV TLSCOH IORDCOH.
     rewrite hb_covered; basic_solver 10.
   Qed.
 
   Lemma dom_urr_covered l:
     dom_rel (urr l ⨾ ⦗ covered T ⦘) ⊆₁ issued T.
-  Proof using WF IMMCON RELCOV TLSCOH IORDCOH.
+  Proof using WF RELCOV TLSCOH IORDCOH WFSC.
     unfold CombRelations.urr.
     generalize dom_rf_covered.
     generalize dom_sc_covered.
@@ -1212,14 +1334,14 @@ Definition issuable T :=
 
   Lemma urr_covered l:
     urr l ⨾ ⦗ covered T ⦘ ⊆ ⦗issued T⦘ ⨾ urr l.
-  Proof using WF IMMCON RELCOV TLSCOH IORDCOH.
+  Proof using WF WFSC RELCOV TLSCOH IORDCOH.
     rewrite (dom_rel_helper (@dom_urr_covered l)).
     basic_solver.
   Qed.
 
   Lemma dom_c_acq_covered i l A:
     dom_rel (c_acq i l A ⨾ ⦗ covered T ⦘) ⊆₁ issued T.
-  Proof using WF IMMCON RELCOV TLSCOH IORDCOH. 
+  Proof using WF WFSC RELCOV TLSCOH IORDCOH. 
     unfold CombRelations.c_acq.
     generalize (@dom_urr_covered l).
     generalize dom_release_issued.
@@ -1229,14 +1351,14 @@ Definition issuable T :=
 
   Lemma c_acq_covered i l A:
     c_acq i l A ⨾ ⦗ covered T ⦘ ⊆ ⦗issued T⦘ ⨾ c_acq i l A.
-  Proof using WF IMMCON  RELCOV TLSCOH IORDCOH.
+  Proof using WF WFSC RELCOV TLSCOH IORDCOH.
     rewrite (dom_rel_helper (@dom_c_acq_covered i l A)).
     basic_solver.
   Qed.
 
   Lemma dom_c_cur_covered i l A:
     dom_rel (c_cur i l A ⨾ ⦗ covered T ⦘) ⊆₁ issued T.
-  Proof using WF IMMCON  RELCOV TLSCOH IORDCOH.
+  Proof using WF WFSC RELCOV TLSCOH IORDCOH.
     unfold CombRelations.c_cur.
     generalize (@dom_urr_covered l).
     basic_solver 21.
@@ -1244,15 +1366,14 @@ Definition issuable T :=
 
   Lemma c_cur_covered i l A:
     c_cur i l A ⨾ ⦗ covered T ⦘ ⊆ ⦗issued T⦘ ⨾ c_cur i l A.
-  Proof using WF IMMCON RELCOV TLSCOH IORDCOH.
+  Proof using WF WFSC RELCOV TLSCOH IORDCOH.
     seq_rewrite (dom_rel_helper (@dom_c_cur_covered i l A)).
     basic_solver.
   Qed.
 
-
   Lemma dom_c_rel_covered i l l' A:
     dom_rel (c_rel i l l' A ⨾ ⦗ covered T ⦘) ⊆₁ issued T.
-  Proof using WF IMMCON RELCOV TLSCOH IORDCOH. 
+  Proof using WF WFSC RELCOV TLSCOH IORDCOH. 
     unfold CombRelations.c_rel.
     generalize (@dom_urr_covered l).
     basic_solver 21.
@@ -1260,14 +1381,14 @@ Definition issuable T :=
 
   Lemma c_rel_covered i l l' A:
     c_rel i l l' A ⨾ ⦗ covered T ⦘ ⊆ ⦗issued T⦘ ⨾ c_rel i l l' A.
-  Proof using WF IMMCON RELCOV TLSCOH IORDCOH. 
+  Proof using WF WFSC RELCOV TLSCOH IORDCOH. 
     seq_rewrite (dom_rel_helper (@dom_c_rel_covered i l l' A)).
     basic_solver.
   Qed.
 
   Lemma t_acq_covered l thread:
     t_acq thread l (covered T) ⊆₁ issued T.
-  Proof using WF IMMCON RELCOV TLSCOH IORDCOH.
+  Proof using WF WFSC RELCOV TLSCOH IORDCOH.
     unfold CombRelations.t_acq.
     rewrite (dom_r (wf_c_acqD G sc thread l (covered T))).
     arewrite (⦗(Tid_ thread ∪₁ Init) ∩₁ covered T⦘ ⊆ ⦗covered T⦘) by basic_solver.
@@ -1277,21 +1398,21 @@ Definition issuable T :=
 
   Lemma t_cur_covered l thread:
     t_cur thread l (covered T) ⊆₁ issued T.
-  Proof using WF IMMCON RELCOV TLSCOH IORDCOH. 
+  Proof using WF WFSC RELCOV TLSCOH IORDCOH. 
     etransitivity; [by apply t_cur_in_t_acq|].
       by apply t_acq_covered.
   Qed.
 
   Lemma t_rel_covered l l' thread:
     t_rel thread l l' (covered T) ⊆₁ issued T.
-  Proof using WF IMMCON RELCOV TLSCOH IORDCOH.
+  Proof using WF WFSC RELCOV TLSCOH IORDCOH.
     etransitivity; [by apply t_rel_in_t_cur|].
       by apply t_cur_covered.
   Qed.
 
   Lemma S_tm_covered l :
     S_tm l (covered T) ⊆₁ issued T.
-  Proof using WF RELCOV IMMCON TLSCOH IORDCOH. 
+  Proof using WF RELCOV TLSCOH IORDCOH. 
     unfold CombRelations.S_tm, CombRelations.S_tmr.
     generalize dom_hb_covered.
     generalize w_covered_issued.
@@ -1302,7 +1423,7 @@ Definition issuable T :=
 
   Lemma msg_rel_issued l:
     dom_rel (msg_rel l ⨾ ⦗ issued T ⦘) ⊆₁ issued T.
-  Proof using WF IMMCON RELCOV TLSCOH IORDCOH.
+  Proof using WF WFSC RELCOV TLSCOH IORDCOH.
     unfold CombRelations.msg_rel.
     generalize dom_release_issued.
     generalize (@dom_urr_covered l).
@@ -1314,9 +1435,52 @@ Section HbProps.
 Notation "'C'" := (covered T).
 Notation "'I'" := (issued  T).
 
+(* TODO: move upper *)
+Lemma ar_int_ct_issuable_in_I:
+  dom_rel (⦗W⦘ ⨾ (ar_int G)^+ ⨾ ⦗issuable T⦘) ⊆₁ I. 
+Proof using WF TLSCOH.
+  unfold issuable. rewrite id_inter with (s := _ ∩₁ _). rewrite <- !seqA. 
+  apply dom_rel_iord_ext_parts.
+  3: { rewrite init_issued. basic_solver. }
+  2: { rewrite ar_int_in_sb, ct_of_trans, wf_sbE, no_sb_to_init; try basic_solver.
+       apply sb_trans. }
+  transitivity (AR G sc); [| unfold iord_simpl; basic_solver 10].
+  unfold AR. hahn_frame. apply map_rel_mori; [done| ].
+  erewrite eqv_rel_mori with (x := _ ∩₁ W); [| intro; apply proj2].
+  hahn_frame. apply clos_trans_mori. unfold ar. basic_solver. 
+Qed.
+
+Lemma rfe_ar_int_ct_issuable_in_I:
+  dom_rel (⦗W⦘ ⨾ (rfe ∪ ar_int G)⁺ ⨾ ⦗issuable T⦘) ⊆₁ I. 
+Proof using WF TLSCOH IORDCOH.
+  rewrite unionC. rewrite path_ut_first.
+  repeat case_union _ _ . rewrite dom_union. apply set_subset_union_l. split.
+  { apply ar_int_ct_issuable_in_I. }
+  
+  rewrite !seqA.
+  assert (dom_rel (rfe ⨾ (ar_int G ∪ rfe)＊ ⨾ ⦗issuable T⦘) ⊆₁ (issued T)) as D.
+  { unfold issuable. rewrite id_inter with (s := _ ∩₁ _). rewrite <- !seqA. 
+    apply dom_rel_iord_ext_parts.
+    3: { rewrite init_issued. basic_solver. }
+    2: { rewrite ar_int_in_sb, rfe_in_rf, sb_E_ENI, rf_E_ENI, unionK, <- ct_begin, ct_of_trans; auto.
+         { basic_solver. }
+         apply E_ENI_trans. }
+    transitivity (AR G sc); [| unfold iord_simpl; basic_solver 10].
+    unfold AR. hahn_frame. apply map_rel_mori; [done| ].
+    erewrite eqv_rel_mori with (x := _ ∩₁ W); [| intro; apply proj2].
+    rewrite (dom_l (wf_rfeD WF)) at 1. hahn_frame.
+    arewrite (rfe ⊆ ar_int G ∪ rfe) at 1. rewrite <- ct_begin.
+    apply clos_trans_mori. unfold ar. basic_solver. }
+  apply dom_rel_helper in D. rewrite D.
+  rewrite <- !seqA. do 3 rewrite dom_seq. rewrite !seqA. 
+  rewrite rtE. repeat case_union _ _. rewrite dom_union.
+  apply set_subset_union_l. split; [basic_solver| ]. 
+  rewrite issued_in_issuable at 1. apply ar_int_ct_issuable_in_I. 
+Qed.
+
 Lemma sw_in_Csw_sb :
   sw ⨾ ⦗C ∪₁ dom_rel (sb^? ⨾ ⦗ I ⦘)⦘ ⊆ ⦗ C ⦘ ⨾ sw ∪ sb.
-Proof using WF RELCOV IMMCON TLSCOH IORDCOH.
+Proof using WF RELCOV TLSCOH IORDCOH.
   rewrite !id_union. rewrite seq_union_r. 
   unionL.
   { rewrite sw_covered; eauto. basic_solver. }
@@ -1348,12 +1512,13 @@ Proof using WF RELCOV IMMCON TLSCOH IORDCOH.
     arewrite (Acq ⊆₁ Acq/Rel) by mode_solver.
     rewrite sb_from_f_in_bob. rewrite bob_in_ar_int. eauto with hahn. }
   seq_rewrite ct_cr.
-  arewrite (rfe ∪ ar_int G ⊆ ar). by apply ar_ct_I_in_I.
+  rewrite issued_in_issuable at 1. 
+  apply rfe_ar_int_ct_issuable_in_I. 
 Qed.
 
 Lemma hb_in_Chb_sb :
   hb ⨾ ⦗C ∪₁ dom_rel (sb^? ⨾ ⦗ I ⦘)⦘ ⊆ ⦗ C ⦘ ⨾ hb ∪ sb.
-Proof using WF RELCOV IMMCON TLSCOH IORDCOH. 
+Proof using WF RELCOV TLSCOH IORDCOH. 
   unfold imm_s_hb.hb.
   intros x y HH.
   destruct_seq_r HH as DOM.
